* Continuation in topography
** Homotopy 
   +---------------------------------------------+
   $m_{k}$                   $k$-th topography 
   $F(\bvec{x},m_{s}) = 0$   starting solution
   $F(\bvec{x},m_{d}) = 0$   destination solution
   +---------------------------------------------+
   Homotopy function:
   $F^h(\bvec{x},\delta) = \hat{\delta} F(\bvec{x},m_d) + (1-\hat{\delta}) F(\bvec{x},m_s)$
   $s = \texttt{floor}(\delta)$ 
   $d = s + 1$
   $\hat{\delta} = \delta - s$

   Or:
   $F^h(\bvec{x}, \delta) = \text{sin}^2(\frac{\pi \delta}{2})F(\bvec{x},m_{d}) + \text{cos}^2(\frac{\pi \delta}{2}) F(\bvec{x},m_{s})$

   delta            = 0..1..2..3..4..5..6..7 
   d                = 1  1  2  2  3  3  4  4
   s                = 0  1  1  2  2  3  3  4
   floor(delta) % 2 = 0  1  0  1  0  1  0  1

   d_{k+1} = d_k + floor(delta) % 2

   $k(\delta) = \texttt{floor}(\delta)$ 
   
   +---------------------------------------------+
   Pseudo-arclength continuation:
   \begin{align*}
   F^h(\bvec{x},\delta) &= 0\\
   \dot{\bvec{x}} (\bvec{x} - \bvec{x}_0) + \dot{\delta} (\delta - \delta_0) - \Delta s &= 0
   \end{align*}
   +---------------------------------------------+   
	
   \begin{equation*}
   \begin{bmatrix}
   F^h_{\bvec{x}} & F^h_{\delta} \\
   \dot{\bvec{x}}^T & \dot{\lambda}   
   \end{bmatrix} \begin{bmatrix} \Delta x \\ \Delta \delta \end{bmatrix} = 
   \begin{bmatrix} -F^h(\bvec{x},\delta) \\ r \end{bmatrix}
   \end{equation*}  
   
   \begin{align*}
   F^h_{\bvec{x}} &= \hat{\delta} F_\bvec{x}(\bvec{x},m_{k+1}) + (1-\hat{\delta}) F_\bvec{x}(\bvec{x},m_{k}) \\
   F^h_{\delta} &=  
   \end{align*}

* Implementation
  
